research/lean_only_proto/DumbContracts/Examples.lean
@@ -10,6 +10,7 @@ import DumbContracts.Examples.NonZeroStore
 import DumbContracts.Examples.CompareAndSwap
 import DumbContracts.Examples.InitOnce
 import DumbContracts.Examples.SetIfGreater
+import DumbContracts.Examples.SetIfAtLeast
 import DumbContracts.Examples.SetIfLess
 import DumbContracts.Examples.SetIfBetween
 import DumbContracts.Examples.AddIfBetween
